% ===============================
%          Chapter 2.2
%      Completing the Square
%     Created by Michael Tang
%           2025.02.24
% ===============================

\subsection{Completing the Square}
A quadratic expression $ax^2 + bx + c$ can be rewritten by completing the square:
\begin{equation}
    x^2 + bx = \left(x + \frac{b}{2}\right)^2 - \left(\frac{b}{2}\right)^2
\end{equation}
This method is useful to express quadratic equations in the form \footnote{Step by step transformation of $ax^2 + bx + c$ to
$a(x - h)^2 + k$:
\begin{equation*}
    \begin{aligned}
        ax^2 + bx + c &= a\left(x^2 + \frac{b}{a}x\right) + c \\
        &= a\left(x^2 + \frac{b}{a}x + \frac{b^2}{4a^2}\right) - \frac{b^2}{4a} + c \\
        &= a\left(x + \frac{b}{2a}\right)^2 - \frac{b^2 - 4ac}{4a} \\
        &= a(x - h)^2 + k
    \end{aligned}
\end{equation*}
where:
\begin{itemize}
    \item $h = -\frac{b}{2a}$
    \item $k = c - \frac{b^2}{4a}$
\end{itemize}}:
\begin{equation}
    a(x - h)^2 + k
\end{equation}
From here, we can easily solve for $x$ by taking the square root of both sides.