% ===============================
%          Chapter 2.1
%   Solving Quadratic Equations
%     Created by Michael Tang
%           2025.02.24
% ===============================

\subsection{Solving Quadratic Equations}
Quadratic equation is in the form:
\begin{equation}
    ax^2 + bx + c = 0
\end{equation}
where $a$, $b$, and $c$ are constants, and $a \neq 0$.

\paragraph{Methods for Solving Quadratics}
\begin{itemize}
    \item[1.] \textbf{Factoring}
    \begin{itemize}
        \item Rearrange the equation into the form $ax^2 + bx + c = 0$.
        \item Factor the left-hand side of the equation.
        \item Set each factor equal to zero and solve for $x$.
    \end{itemize}
    \item[2.] \textbf{Using the Quadratic Formula} \footnote{Step by step transformation from the standard quadratic equation
    $ax^2 + bx + c = 0$ to the quadratic formula:
    \begin{equation*}
        \begin{aligned}
            ax^2 + bx + c &= 0 \\
            x^2 + \frac{b}{a}x + \frac{c}{a} &= 0 \\
            x^2 + \frac{b}{a}x &= -\frac{c}{a} \\
            x^2 + \frac{b}{a}x + \left(\frac{b}{2a}\right)^2 &= -\frac{c}{a} + \left(\frac{b}{2a}\right)^2 \\
            \left(x + \frac{b}{2a}\right)^2 &= \frac{b^2 - 4ac}{4a^2} \\
            x + \frac{b}{2a} &= \pm \sqrt{\frac{b^2 - 4ac}{4a^2}} \\
            x &= \frac{-b \pm \sqrt{b^2 - 4ac}}{2a}
        \end{aligned}
    \end{equation*}} The solution are given by the formula:
    \begin{equation}
        x = \frac{-b \pm \sqrt{b^2 - 4ac}}{2a}
    \end{equation}
    where $a$, $b$, and $c$ are the coefficients from the quadratic equation $ax^2 + bx + c = 0$.
\end{itemize}